More cleaning

experiments/dm4ms/MST.fst
@@ -16,80 +16,19 @@ module W = FStar.Monotonic.Witnessed
 
 (** ** START Section 1: specification monad **)
 
-(** Preconditions are predicates on the [heap] *)
-let st_pre_h (heap: Type) = heap -> GTot Type0
-
-(** Postconditions relate [a]-typed results to the final [heap], here
-    refined by some pure proposition [pre], typically instantiated to
-    the precondition applied to the initial [heap] *)
-let st_post_h' (heap a pre: Type) = a -> _: heap{pre} -> GTot Type0
-
-(** Postconditions without refinements *)
-let st_post_h (heap a: Type) = st_post_h' heap a True
-
+(** Most of it defined in FStar.Pervasives, here just adding monotonicity *)
 unfold
 let st_post_ord (#heap:Type) (p1 p2:st_post_h heap 'a) =
   forall r h. p1 r h ==> p2 r h
 
-(** The type of the main WP-transformer for stateful computations *)
-let st_wp_h0 (heap a: Type) = st_post_h heap a -> Tot (st_pre_h heap)
-
 unfold
-let st_wp_monotonic (heap:Type) (wp:st_wp_h0 heap 'a) =
+let st_wp_monotonic (heap:Type) (wp:st_wp_h heap 'a) =
   forall p1 p2. (p1 `st_post_ord` p2) ==> (forall h. wp p1 h ==> wp p2 h)
 
-(** !!! This is the only difference to the monad used by F* state, the fact that
-  here st_wp_h has to be monotonic *)
-let st_wp_h (heap a: Type) = wp:(st_wp_h0 heap a){st_wp_monotonic heap wp}
-
-(** Returning a value does not transform the state *)
-unfold
-let st_return (heap:Type u#b) (a: Type u#a) (x: a) (p: st_post_h heap a) = p x
-
-(** Sequential composition of stateful WPs *)
-unfold
-let st_bind_wp
-      (heap: Type u#c)
-      (a:Type u#a)
-      (b: Type u#b)
-      (wp1: st_wp_h heap a)
-      (wp2: (a -> GTot (st_wp_h heap b)))
-      (p: st_post_h heap b)
-      (h0: heap)
-     = wp1 (fun a h1 -> wp2 a p h1) h0
-
-(** Branching for stateful WPs *)
-unfold
-let st_if_then_else
-      (heap a p: Type)
-      (wp_then wp_else: st_wp_h heap a)
-      (post: st_post_h heap a)
-      (h0: heap)
-     = wp_then post h0 /\ (~p ==> wp_else post h0)
-
-(** As with [PURE] the [wp] combinator names the postcondition as
-    [k] to avoid duplicating it. *)
-unfold
-let st_ite_wp (heap a: Type) (wp: st_wp_h heap a) (post: st_post_h heap a) (h0: heap) =
-  forall (k: st_post_h heap a).
-    (forall (x: a) (h: heap). {:pattern (guard_free (k x h))} post x h ==> k x h) ==> wp k h0
-
-(** Subsumption for stateful WPs *)
-unfold
-let st_stronger (heap a: Type) (wp1 wp2: st_wp_h heap a) =
-  (forall (p: st_post_h heap a) (h: heap). wp1 p h ==> wp2 p h)
+let st_wp (heap a: Type) = wp:(st_wp_h heap a){st_wp_monotonic heap wp}
 
 unfold
 let (⊑) #heap #a wp1 wp2 = st_stronger heap a wp2 wp1
-
-(** Closing the scope of a binder within a stateful WP *)
-unfold
-let st_close_wp (heap a b: Type) (wp: (b -> GTot (st_wp_h heap a))) (p: st_post_h heap a) (h: heap) =
-  (forall (b: b). wp b p h)
-
-(** Applying a stateful WP to a trivial postcondition *)
-unfold
-let st_trivial (heap a: Type) (wp: st_wp_h heap a) = (forall h0. wp (fun r h1 -> True) h0)
 (** ** END Section 1: specification monad **)
 
 
@@ -133,28 +72,28 @@ let rec free_bind
 
 (** ** START Section 3: theta **)
 unfold
-let partial_call_wp (#state:tstate) (pre:pure_pre) : st_wp_h state.t (squash pre) = 
-  let wp' : st_wp_h0 state.t (squash pre) = fun p h0 -> pre /\ p () h0 in
+let partial_call_wp (#state:tstate) (pre:pure_pre) : st_wp state.t (squash pre) = 
+  let wp' : st_wp_h state.t (squash pre) = fun p h0 -> pre /\ p () h0 in
   assert (st_wp_monotonic state.t wp');
   wp'
 
 unfold
-let get_wp (#state:tstate) : st_wp_h state.t state.t =
+let get_wp (#state:tstate) : st_wp state.t state.t =
   fun p h0 -> p h0 h0
 
 unfold
-let put_wp (#state:tstate) (h1:state.t) : st_wp_h state.t unit =
+let put_wp (#state:tstate) (h1:state.t) : st_wp state.t unit =
   fun p h0 -> (h0 `state.rel` h1) /\ p () h1
 
 unfold
-let witness_wp (#state:tstate) (pred:state.t -> Type0) : st_wp_h state.t unit =
+let witness_wp (#state:tstate) (pred:state.t -> Type0) : st_wp state.t unit =
   fun p h -> pred h /\ FStar.Preorder.stable pred state.rel /\ (W.witnessed state.rel pred ==> p () h)
 
 unfold
-let recall_wp (#state:tstate) (pred:state.t -> Type0) : st_wp_h state.t unit =
+let recall_wp (#state:tstate) (pred:state.t -> Type0) : st_wp state.t unit =
   fun p h -> W.witnessed state.rel pred /\ (pred h ==> p () h)
 
-val theta : #a:Type u#a -> #state:tstate u#s -> free state a -> st_wp_h state.t a
+val theta : #a:Type u#a -> #state:tstate u#s -> free state a -> st_wp state.t a
 let rec theta #a #state m =
   match m with
   | Return x -> st_return state.t _ x
@@ -269,7 +208,7 @@ let rec lemma_theta_is_lax_morphism_bind
 (** ** END Section 3: theta **)
 
 (** ** START Section 4: Dijkstra Monad **)
-let mst (state:tstate) (a:Type) (wp:st_wp_h state.t a)=
+let mst (state:tstate) (a:Type) (wp:st_wp state.t a)=
   m:(free state a){theta m ⊑ wp}
 
 let mst_return (#state:tstate) (#a:Type) (x:a) : mst state a (st_return state.t _ x) =
@@ -279,8 +218,8 @@ let mst_bind
   (#state:tstate u#s)
   (#a : Type u#a)
   (#b : Type u#b)
-  (#wp_v : st_wp_h state.t a)
-  (#wp_f: a -> st_wp_h state.t b)
+  (#wp_v : st_wp state.t a)
+  (#wp_f: a -> st_wp state.t b)
   (v : mst state a wp_v)
   (f : (x:a -> mst state b (wp_f x))) :
   Tot (mst state b (st_bind_wp state.t a b wp_v wp_f)) =
@@ -290,8 +229,8 @@ let mst_bind
 let mst_subcomp
   (#state:tstate u#s)
   (#a : Type u#a)
-  (#wp1 : st_wp_h state.t a)
-  (#wp2 : st_wp_h state.t a)
+  (#wp1 : st_wp state.t a)
+  (#wp2 : st_wp state.t a)
   (v : mst state a wp1)
   :
   Pure (mst state a wp2) (requires (wp1 ⊑ wp2)) (ensures (fun _ -> True)) =
